use sha2_256 from code/hash

specs/Spec.RSAPSS.fst
@@ -9,7 +9,6 @@ open Lib.ByteSequence
 open Lib.LoopCombinators
 open Lib.NatMod
 
-module Hash = Spec.Agile.Hash
 
 #reset-options "--z3rlimit 50 --max_fuel 0 --max_ifuel 0"
 
@@ -17,62 +16,43 @@ module Hash = Spec.Agile.Hash
 /// Auxillary functions
 ///
 
-let size_pos = x:size_nat{x > 0}
-
-val blocks:
-    x: size_pos
-  -> m: size_pos ->
-  Tot (r:size_pos{x <= m * r})
-
+val blocks: x: size_pos -> m: size_pos -> Tot (r:size_pos{x <= m * r})
 let blocks x m = (x - 1) / m + 1
 
+val xor_bytes: #len: size_pos -> b1: lbytes len -> b2: lbytes len -> Tot (lbytes len)
+let xor_bytes #len b1 b2 = map2 (fun x y -> x ^. y) b1 b2
 
-val xor_bytes:
-    #len: size_pos
-  -> b1: lbytes len
-  -> b2: lbytes len ->
-  Tot (lbytes len)
+let hLen = 32
+let max_input = Spec.Hash.Definitions.max_input_length Spec.Hash.Definitions.SHA2_256
+let sha2_256 (msg:bytes{length msg < max_input}) : lbytes hLen = Spec.Hash.hash Spec.Hash.Definitions.SHA2_256 msg
 
-let xor_bytes #len b1 b2 =
-  map2 (fun x y -> x ^. y) b1 b2
-
-let hLen = Spec.Agile.Hash.size_hash Spec.Agile.Hash.HASH_SHA2_256
 
 (* Mask Generation Function *)
 val mgf_sha256:
-    #len: size_nat{len + 4 <= max_size_t /\ len + 4 <= Spec.Agile.Hash.max_input Spec.Agile.Hash.HASH_SHA2_256}
+    #len: size_nat{len + 4 <= max_size_t /\ len + 4 < max_input}
   -> mgfseed: lbytes len
   -> maskLen: size_pos{(blocks maskLen hLen) * hLen < pow2 32} ->
   Tot (lbytes maskLen)
 
 let mgf_sha256 #len mgfseed maskLen =
-  let n = blocks maskLen hLen in
-  let acc = create (n * hLen) (u8 0) in
   let mgfseed_counter = create (len + 4) (u8 0) in
   let mgfseed_counter = update_sub mgfseed_counter 0 len mgfseed in
-  let acc =
-    repeati n (fun i acc ->
-      let counter = nat_to_bytes_be 4 i in
-      let mgfseed_counter = update_sub mgfseed_counter len 4 counter in
-      let mHash = Spec.Agile.Hash.hash Spec.Agile.Hash.HASH_SHA2_256 mgfseed_counter in
-      update_sub acc (hLen * i) hLen mHash
-    ) acc in
-  sub acc 0 maskLen
+
+  let f (i:size_nat) : lbytes hLen =
+    let counter = nat_to_bytes_be 4 i in
+    let mgfseed_counter = update_sub mgfseed_counter len 4 counter in
+    sha2_256 mgfseed_counter in
+
+  let n = blocks maskLen hLen in
+  let acc = generate_blocks_simple #uint8 hLen n n f in
+  sub #uint8 #(n * hLen) acc 0 maskLen
+
 
 (* Bignum convert functions *)
-val os2ip:
-    #len: size_nat
-  -> b: lbytes len ->
-  Tot (res: nat{res < pow2 (8 * len)})
-
+val os2ip: #len: size_nat -> b: lbytes len -> Tot (res: nat{res < pow2 (8 * len)})
 let os2ip #len b = nat_from_bytes_be b
 
-
-val i2osp:
-    #len: size_nat
-  -> n: nat{n < pow2 (8 * len)} ->
-  Tot (lbytes len)
-
+val i2osp: #len: size_nat -> n: nat{n < pow2 (8 * len)} -> Tot (lbytes len)
 let i2osp #len n = nat_to_bytes_be len n
 
 
@@ -83,7 +63,7 @@ let i2osp #len n = nat_to_bytes_be len n
 type modBits = modBits: size_nat{1 < modBits}
 
 noeq type rsa_pubkey (modBits:modBits) =
-  | Mk_rsa_pubkey: n: nat{1 < n /\ pow2 (modBits - 1) <= n /\ n < pow2 modBits}
+  | Mk_rsa_pubkey: n: nat{pow2 (modBits - 1) <= n /\ n < pow2 modBits}
                  -> e: nat_mod n{1 < nat_mod_v e}
                  -> rsa_pubkey modBits
 
@@ -92,12 +72,7 @@ noeq type rsa_privkey (modBits:modBits) =
                   -> d: nat_mod (Mk_rsa_pubkey?.n pkey){1 < nat_mod_v d}
                   -> rsa_privkey modBits
 
-val db_zero:
-    #len: size_pos
-  -> db: lbytes len
-  -> emBits: size_nat ->
-  Tot (lbytes len)
-
+val db_zero: #len: size_pos -> db: lbytes len -> emBits: size_nat -> Tot (lbytes len)
 let db_zero #len db emBits =
   let msBits = emBits % 8 in
   if msBits > 0 then
@@ -105,22 +80,22 @@ let db_zero #len db emBits =
   else db
 
 val pss_encode:
-    #sLen: size_nat{sLen + hLen + 8 < max_size_t /\ sLen + hLen + 8 <= Spec.Agile.Hash.max_input Spec.Agile.Hash.HASH_SHA2_256}
-  -> #msgLen: size_nat{msgLen <= Spec.Agile.Hash.max_input Spec.Agile.Hash.HASH_SHA2_256}
+    #sLen: size_nat{sLen + hLen + 8 < max_size_t /\ sLen + hLen + 8 < max_input}
+  -> #msgLen: size_nat{msgLen < max_input}
   -> salt: lbytes sLen
   -> msg: lbytes msgLen
   -> emBits: size_pos{hLen + sLen + 2 <= blocks emBits 8} ->
   Tot (lbytes (blocks emBits 8))
 
 let pss_encode #sLen #msgLen salt msg emBits =
-  let mHash = Spec.Agile.Hash.hash Spec.Agile.Hash.HASH_SHA2_256 msg in
+  let mHash = sha2_256 msg in
 
   //m1 = [8 * 0x00; mHash; salt]
   let m1Len = 8 + hLen + sLen in
   let m1 = create m1Len (u8 0) in
   let m1 = update_sub m1 8 hLen mHash in
   let m1 = update_sub m1 (8 + hLen) sLen salt in
-  let m1Hash = Spec.Agile.Hash.hash Spec.Agile.Hash.HASH_SHA2_256 m1 in
+  let m1Hash = sha2_256 m1 in
 
   //db = [0x00;..; 0x00; 0x01; salt]
   let emLen = blocks emBits 8 in
@@ -130,7 +105,7 @@ let pss_encode #sLen #msgLen salt msg emBits =
   let db = db.[last_before_salt] <- u8 1 in
   let db = update_sub db (last_before_salt + 1) sLen salt in
 
-  let dbMask = mgf_sha256 #(length m1Hash) m1Hash dbLen in
+  let dbMask = mgf_sha256 #hLen m1Hash dbLen in
   let maskedDB = xor_bytes db dbMask in
   let maskedDB = db_zero maskedDB emBits in
 
@@ -142,15 +117,15 @@ let pss_encode #sLen #msgLen salt msg emBits =
 
 
 val pss_verify:
-    #msgLen: size_nat{msgLen <= Spec.Agile.Hash.max_input Spec.Agile.Hash.HASH_SHA2_256}
-  -> sLen: size_nat{sLen + hLen + 8 <= max_size_t /\ sLen + hLen + 8 <= Spec.Agile.Hash.max_input Spec.Agile.Hash.HASH_SHA2_256}
+    #msgLen: size_nat{msgLen < max_input}
+  -> sLen: size_nat{sLen + hLen + 8 <= max_size_t /\ sLen + hLen + 8 < max_input}
   -> msg: lbytes msgLen
   -> emBits: size_pos
   -> em: lbytes (blocks emBits 8) ->
   Tot bool
 
 let pss_verify #msgLen sLen msg emBits em =
-  let mHash = Spec.Agile.Hash.hash Spec.Agile.Hash.HASH_SHA2_256 msg in
+  let mHash = sha2_256 msg in
 
   let emLen = blocks emBits 8 in
   let msBits = emBits % 8 in
@@ -179,20 +154,20 @@ let pss_verify #msgLen sLen msg emBits em =
 
       if not (lbytes_eq pad pad2) then false
       else begin
-	     let m1Len = 8 + hLen + sLen in
-	     let m1 = create m1Len (u8 0) in
-	     let m1 = update_sub m1 8 hLen mHash in
-	     let m1 = update_sub m1 (8 + hLen) sLen salt in
-	     let m1Hash0 = Spec.Agile.Hash.hash Spec.Agile.Hash.HASH_SHA2_256 m1 in
-	     lbytes_eq m1Hash0 m1Hash
+        let m1Len = 8 + hLen + sLen in
+        let m1 = create m1Len (u8 0) in
+        let m1 = update_sub m1 8 hLen mHash in
+        let m1 = update_sub m1 (8 + hLen) sLen salt in
+        let m1Hash0 = sha2_256 m1 in
+        lbytes_eq m1Hash0 m1Hash
       end
     end
   end
 
 
 val rsapss_sign:
-    #sLen: size_nat{sLen + hLen + 8 <= max_size_t /\ sLen + hLen + 8 <= Spec.Agile.Hash.max_input Spec.Agile.Hash.HASH_SHA2_256}
-  -> #msgLen: size_nat{msgLen <= Spec.Agile.Hash.max_input Spec.Agile.Hash.HASH_SHA2_256}
+    #sLen: size_nat{sLen + hLen + 8 <= max_size_t /\ sLen + hLen + 8 < max_input}
+  -> #msgLen: size_nat{msgLen < max_input}
   -> modBits: modBits{sLen + hLen + 2 <= blocks (modBits - 1) 8}
   -> skey: rsa_privkey modBits
   -> salt: lbytes sLen
@@ -220,10 +195,10 @@ let rsapss_sign #sLen #msgLen modBits skey salt msg =
 
 
 val rsapss_verify:
-    #msgLen: size_nat{msgLen <= Spec.Agile.Hash.max_input Spec.Agile.Hash.HASH_SHA2_256}
+    #msgLen: size_nat{msgLen < max_input}
   -> modBits: modBits
   -> pkey: rsa_pubkey modBits
-  -> sLen: size_nat{sLen + hLen + 8 <= max_size_t /\ sLen + hLen + 8 <= Spec.Agile.Hash.max_input Spec.Agile.Hash.HASH_SHA2_256}
+  -> sLen: size_nat{sLen + hLen + 8 <= max_size_t /\ sLen + hLen + 8 < max_input}
   -> msg: lbytes msgLen
   -> sgnt: lbytes (blocks modBits 8) ->
   Tot bool
